src/absyn/syntax.fs
@@ -18,6 +18,7 @@ module Microsoft.FStar.Absyn.Syntax
 (* Type definitions for the core AST *)
 
 open Microsoft.FStar
+open Microsoft.FStar.ML
 open Microsoft.FStar.Util
 
 exception Err of string
@@ -73,7 +74,7 @@ type typ' =
   | Typ_unknown                                              (* not present after 1st round tc *)
 and typ = {t:typ'; k:knd}
 and comp_typ = 
-  | Computation of (lident * typ * typ)
+  | Computation of typ
   | Pure of typ
 and uvar_t = Unionfind.uvar<uvar_basis<typ,knd>>
 and meta_t = 
@@ -157,6 +158,29 @@ type atag =
   | Definition
   | Lemma
 
+type monad_abbrev = {
+  mabbrev:lident;
+  parms:list<tparam>;
+  def:typ
+  }
+type monad_decl = {
+    mname:lident;
+    total:bool;
+    signature:knd;
+    ret:typ;
+    bind_wp:typ;
+    bind_wlp:typ;
+    ite_wp:typ;
+    ite_wlp:typ;
+    abbrevs:list<monad_abbrev>
+  }
+type monad_order = {
+  source:lident;
+  target:lident;
+  lift: typ
+ }
+type monad_lat = list<monad_order>
+
 type sigelt =
   | Sig_tycon          of lident * list<tparam> * knd * list<lident> * list<lident> * list<logic_tag> * Range.range (* bool is for a prop, list<lident> identifies mutuals, second list<lident> are all the constructors *)
   | Sig_typ_abbrev     of lident * list<tparam> * knd * typ * Range.range 
@@ -167,6 +191,7 @@ type sigelt =
   | Sig_let            of letbindings * Range.range 
   | Sig_main           of exp * Range.range 
   | Sig_bundle         of list<sigelt> * Range.range  (* an inductive type is a bundle of all mutually defined Sig_tycons and Sig_datacons *)
+  | Sig_monads         of list<monad_decl> * monad_lat
 type sigelts = list<sigelt>
 
 type modul = {
